Test/dafny0/ResolutionErrors.dfy
@@ -8,18 +8,82 @@ method GhostDivergentLoop()
    ghost var i := 0;
    while (i < 2)
       decreases *; // error: not allowed on a ghost loop
-	  invariant i <= 2;
-	  invariant (forall j :: 0 <= j && j < i ==> a[j] > 0);
+      invariant i <= 2;
+      invariant (forall j :: 0 <= j && j < i ==> a[j] > 0);
    {
      i := 0;
    }
    assert a[1] != a[1]; // ...for then this would incorrectly verify
 }
 
-method M<T>(a: array3<T>, b: array<T>, m: int, n: int)
+method ManyIndices<T>(a: array3<T>, b: array<T>, m: int, n: int)
 {
   // the following invalid expressions were once incorrectly resolved:
   var x := a[m, n];        // error
   var y := a[m];           // error
   var z := b[m, n, m, n];  // error
+}
+
+// -------- name resolution
+
+class Global {
+  var X: int;
+  function method F(x: int): int { x }
+  static function method G(x: int): int { x }
+  method M(x: int) returns (r: int)
+  {
+    r := x + X;
+  }
+  static method N(x: int) returns (r: int)
+  {
+    r := x + X;  // error: cannot access instance field X from static method
+  }
+}
+
+method TestNameResolution0() {
+  var z: int;
+  z := Global.X;  // error: X is an instance field
+  z := F(2);  // error: cannot resolve F
+  z := Global.F(2);  // error: invocation of instance function requires an instance
+  z := G(2);  // error: cannot resolve G
+  z := Global.G(2);
+  call z := M(2);  // error: cannot resolve M
+//  call z := Global.M(2);  // error: call to instance method requires an instance
+  call z := N(1);  // error: cannot resolve N
+//  call z := Global.N(1);
+
+  z := z(5);  // error: using local as if it were a function
+  z := Global.z;  // error: class Global does not have a member z
+
+  var Global: Global;  // a local variable with the name 'Global'
+  z := Global.X;  // this means the instance field X of the object stored in the local variable 'Global'
+  var gg: Global := null;
+  var y := gg.G(5);
+  call y := gg.N(5);
+}
+
+datatype Abc = Abel | Benny | Cecilia(y: int) | David(x: int) | Eleanor;
+datatype Xyz = Alberta | Benny | Constantine(y: int) | David(x: int);
+datatype Rst = David(x: int, y: int);
+
+function Tuv(arg0: Abc, arg1: bool): int { 10 }
+var Eleanor: bool;
+
+method TestNameResolution1() {
+  var a0 := Abel;
+  var a1 := Alberta;
+  var b0 := Benny;  // error: there's more than one constructor with the name Benny; needs qualification
+  var b1 := Abc.Benny;
+  var b2 := Xyz.Benny;
+  var Benny := 15;  // introduce a local variable with the name 'Benny'
+  var b3 := Benny;
+  var d0 := David(20);  // error: constructor name David is ambiguous
+  var d1 := David;  // error: constructor name David is ambiguous (never mind that the signature does
+                    // not match either of them)
+  var d2 := David(20, 40);  // error: constructor name Davis is ambiguous (never mind that the given
+                            // parameters match the signature of only one of those constructors)
+  var d3 := Abc.David(20, 40);  // error: wrong number of parameters
+  var d4 := Rst.David(20, 40);
+  var e := Eleanor;
+  assert Tuv(e, this.Eleanor) == 10;
 }
