Test/dafny0/Basics.dfy
@@ -1,0 +1,44 @@
+class Global {
+  static function G(x: int): int { x+x }
+  static method N(x: int) returns (ghost r: int)
+    ensures r == Global.G(x);
+  {
+    if {
+      case true =>  r := G(x+0);
+      case true =>
+        var g: Global;
+        r := g.G(x);
+      case true =>
+        var g: Global := null;
+        r := g.G(x);
+      case true =>
+        r := Global.G(x);
+    }
+  }
+}
+
+method TestCalls(k: nat) {
+  var g: Global, h: Global;
+  assume g != h;
+  ghost var r: int;
+  ghost var s := Global.G(k);
+
+//  call r := Global.N(k);
+//  assert r == s;
+
+  call r := g.N(k);
+  assert r == s;
+  call r := h.N(k);
+  assert r == s;
+
+  g := null;
+  call r := g.N(k);
+  assert r == s;
+
+//  call r := Global.N(r);
+  if (k == 0) {
+    assert r == s;
+  } else {
+//    assert r == s;  // error: G(k) and G(k+k) are different
+  }
+}
